coq/ApplyTy.v
@@ -3,487 +3,6 @@ Require Import Coq.micromega.Lia.
 Require Import LN_Lemmas.
 Require Export DistSubtyping.
 
-#[export] Hint Extern 1 (lc_typ (t_forall _)) =>
-let Y:= fresh "Y" in pick_fresh Y; instantiate_cofinites_with Y; applys lc_t_forall_exists Y : core.
-
-
-Ltac inv_arrow :=
-  repeat match goal with
-         | H: algo_sub (t_arrow _ _) (t_arrow _ _) |- _ => forwards (?&?): algo_sub_arrow_inv H; clear H
-         | H: declarative_subtyping (t_arrow _ _) (t_arrow _ _) |- _ => apply dsub2asub in H
-         end.
-
-Ltac inv_forall :=
-  repeat match goal with
-         | H: algo_sub (t_forall _) (t_forall _) |- _ => forwards : algo_sub_forall_inv H; clear H
-         | H: declarative_subtyping (t_forall _) (t_forall _) |- _ => apply dsub2asub in H
-         end.
-
-
-Ltac convert2asub :=
-  repeat match goal with
-           H: declarative_subtyping _ _ |- _ => apply dsub2asub in H
-           | |- declarative_subtyping _ _ => apply dsub2asub
-         end.
-
-Ltac convert2dsub :=
-  repeat match goal with
-           | H: algo_sub _ _ |- _ => apply dsub2asub in H
-           | |- algo_sub _ _ => apply dsub2asub
-         end.
-
-Lemma sub_inv_1 : forall X B D,
-    algo_sub (t_tvar_f X) (t_arrow B D) -> False.
-Proof.
-  introv H. indTypSize (size_typ (t_arrow B D)).
-  inverts H; solve_false.
-  all: inverts H0; applys IH; try eassumption; elia.
-Qed.
-
-Lemma sub_inv_2 : forall l5 A B D,
-    algo_sub (t_rcd l5 A) (t_arrow B D) -> False.
-Proof.
-  introv H. indTypSize (size_typ (t_rcd l5 A) + size_typ (t_arrow B D)).
-  inverts H; solve_false.
-  all: inverts H0; applys IH; try eassumption; elia.
-Qed.
-
-Lemma sub_inv_3 : forall B D,
-    algo_sub t_top (t_arrow B D) -> False.
-Proof.
-  introv H. indTypSize (size_typ (t_arrow B D)).
-  inverts H; solve_false.
-  all: inverts H0; applys IH; try eassumption; elia.
-Qed.
-
-Lemma sub_inv_4 : forall A B D,
-    algo_sub (t_forall A) (t_arrow B D) -> False.
-Proof.
-  introv H. indTypSize (size_typ (t_forall A) + size_typ (t_arrow B D)).
-  inverts H; solve_false.
-  all: inverts H0; applys IH; try eassumption; elia.
-Qed.
-
-Lemma sub_inv_5 : forall X B,
-    algo_sub (t_tvar_f X) (t_forall B) -> False.
-Proof.
-  introv H. indTypSize (size_typ (t_forall B)).
-  inverts H; solve_false.
-  all: inverts H0; applys IH; try eassumption; elia.
-Qed.
-
-Lemma sub_inv_6 : forall l5 A B,
-    algo_sub (t_rcd l5 A) (t_forall B) -> False.
-Proof.
-  introv H. indTypSize (size_typ (t_rcd l5 A) + size_typ (t_forall B)).
-  inverts H; solve_false.
-  all: inverts H0; applys IH; try eassumption; elia.
-Qed.
-
-Lemma sub_inv_7 : forall B,
-    algo_sub t_top (t_forall B) -> False.
-Proof.
-  introv H. indTypSize (size_typ (t_forall B)).
-  inverts H; solve_false.
-  all: inverts H0; applys IH; try eassumption; elia.
-Qed.
-
-Lemma sub_inv_8 : forall A B D,
-    algo_sub (t_arrow B D) (t_forall A) -> False.
-Proof.
-  introv H. indTypSize (size_typ (t_forall A) + size_typ (t_arrow B D)).
-  inverts H; solve_false.
-  all: inverts H0; applys IH; try eassumption; elia.
-Qed.
-
-#[export] Hint Extern 1 => match goal with
-   | H: algo_sub (t_tvar_f _) (t_arrow _ _) |- _ => applys sub_inv_1 H
-   | H: algo_sub (t_rcd _ _) (t_arrow _ _) |- _ => applys sub_inv_2 H
-   | H: algo_sub t_top (t_arrow _ _) |- _ => applys sub_inv_3 H
-   | H: algo_sub (t_forall _) (t_arrow _ _) |- _ => applys sub_inv_4 H
-   | H: algo_sub (t_tvar_f _) (t_forall _) |- _ => applys sub_inv_5 H
-   | H: algo_sub (t_rcd _ _) (t_forall _) |- _ => applys sub_inv_6 H
-   | H: algo_sub t_top (t_forall _) |- _ => applys sub_inv_7 H
-   | H: algo_sub (t_arrow _ _) (t_forall _) |- _ => applys sub_inv_8 H
-                            end : FalseHd.
-
-(******** nondeterministic split & alternative subtyping definition *******)
-
-Lemma new_splu_decrease_size: forall A B C,
-    new_splu A B C -> size_typ B < size_typ A /\ size_typ C < size_typ A.
-Proof with (pose proof (size_typ_min); simpl in *; try lia).
-  introv H.
-  induction H; simpl in *; eauto...
-  pick fresh X. forwards* (?&?): H0.
-  rewrite 2 size_typ_open_typ_wrt_typ_var in H3.
-  rewrite 2 size_typ_open_typ_wrt_typ_var in H2.
-  eauto...
-Qed.
-
-Lemma new_spli_decrease_size: forall A B C,
-    new_spli A B C -> size_typ B < size_typ A /\ size_typ C < size_typ A.
-Proof with (pose proof (size_typ_min); simpl in *; try lia).
-  introv H.
-  induction H; simpl in *; eauto...
-  - forwards (?&?): new_splu_decrease_size H0...
-  - pick fresh X. forwards* (?&?): H0.
-    rewrite 2 size_typ_open_typ_wrt_typ_var in H3.
-    rewrite 2 size_typ_open_typ_wrt_typ_var in H2.
-    eauto...
-Qed.
-
-Ltac new_spl_size :=
-  repeat match goal with
-         | [ H: new_splu _ _ _ |- _ ] =>
-           ( lets (?&?): new_splu_decrease_size H; clear H)
-         | [ H: new_spli _ _ _ |- _ ] =>
-           ( lets (?&?): new_spli_decrease_size H; clear H)
-         end.
-
-Ltac new_elia :=
-  try solve [pose proof (size_typ_min);
-             let x := fresh "x" in
-             pick fresh x; instantiate_cofinites_with x; (* forall x, x `notin` .. -> spli .. *)
-             spl_size; new_spl_size; simpl in *; simpl;
-             try repeat rewrite size_typ_open_typ_wrt_typ_var in *; (* spl A-^X ... *)
-             try lia].
-
-(******* relates to original definitions ********)
-
-Lemma splu2nsplu : forall A B1 B2,
-    splu A B1 B2 -> new_splu A B1 B2.
-Proof.
-  introv H. induction* H.
-Qed.
-
-Lemma spli2nspli : forall A B1 B2,
-    spli A B1 B2 -> new_spli A B1 B2.
-Proof.
-  introv H. induction~ H.
-  - apply splu2nsplu in H0. eauto.
-  - econstructor. intros. instantiate_cofinites. easy.
-Qed.
-
-#[export] Hint Resolve splu2nsplu spli2nspli : core.
-
-Notation "A <:: B" := (algo_sub A B) (at level 15).
-Notation "A ~~ B" := ((algo_sub A B) /\ (algo_sub B A)) (at level 15).
-Notation "A & B" := (t_and A B) (at level 10).
-Notation "A | B" := (t_or A B) (at level 11).
-
-Lemma nsplu2splu : forall A B1 B2,
-    new_splu A B1 B2 ->
-    exists C1 C2, splu A C1 C2.
-Proof with destruct_conj; eauto.
-  introv H. induction H...
-  - destruct* (ordu_or_split A)...
-  - pick fresh Y for (L `union` [[A]]). instantiate_cofinites. exists.
-    applys splu_forall_exists Y...
-Qed.
-
-Lemma nspli2spli : forall A B1 B2,
-    new_spli A B1 B2 ->
-    exists C1 C2, spli A C1 C2.
-Proof with destruct_conj; eauto.
-  introv H. induction H...
-  - destruct* (ordi_or_split A)...
-  - destruct* (ordi_or_split B)...
-    + apply nsplu2splu in H0...
-  - pick fresh Y for (L `union` [[A]]). instantiate_cofinites. exists.
-    applys spli_forall_exists Y...
-Qed.
-
-Ltac gets_all_lc :=
-  repeat match goal with
-         | H: ordi _ |- _ => lets: ordi_lc H; assumption
-         | H: ordu _ |- _ => lets: ordi_lc H; assumption
-         | H: splu _ _ _ |- _ => lets (?&?&?): splu_lc H; assumption
-         | H: spli _ _ _ |- _ => lets (?&?&?): spli_lc H; assumption
-         | H: algo_sub _ _ |- _ => lets (?&?): algo_sub_lc H; assumption
-         end.
-
-Lemma open_into_var : forall X Y, t_tvar_f Y -^ X = t_tvar_f Y.
-Proof. eauto. Qed.
-
-Hint Rewrite open_into_var : open.
-
-Lemma nsplu_isomorphic : forall A B1 B2,
-    new_splu A B1 B2 -> A ~~ B1|B2.
-Proof with try applys ASub_refl; try match goal with |- lc_typ _ => eauto with lngen end.
-  introv H. split; induction~ H.
-  - split_r.
-    + swap_or_r... split_r.
-      swap_or_r... applys* ASub_andl. applys* ASub_andr.
-    + applys* ASub_orl.
-  - swap_and_l... split_r.
-    + applys* ASub_orl.
-    + swap_or_r... split_r. applys* ASub_andr.
-      swap_or_r... applys* ASub_andl.
-  - applys algo_trans; [ | applys dsub2asub; applys DSub_CovDistUAll ]...
-    econstructor. intros. instantiate_cofinites.
-    applys algo_trans H0. autorewrite with open.
-    auto.
-  - applys algo_trans; [ | applys dsub2asub; applys DSub_CovDistUIn ]...
-    econstructor. easy.
-  - split_l.
-    + split_r.
-      * use_left_l. applys algo_trans IHnew_splu. use_left_r...
-      * use_right_l...
-    + split_r.
-      * use_left_l. applys algo_trans IHnew_splu. use_right_r...
-      * use_right_l...
-  - split_l.
-    + split_r.
-      * use_left_l...
-      * applys algo_trans IHnew_splu. use_left_r... use_right_l...
-    + split_r.
-      * use_left_l...
-      * applys algo_trans IHnew_splu. use_right_r... use_right_l...
-  - applys algo_trans (t_forall (A1|A2))...
-    + split_l; applys ASub_forall; intros; instantiate_cofinites;
-       autorewrite with open...
-      use_left_r... use_right_r...
-    + applys ASub_forall; intros; instantiate_cofinites;
-       autorewrite with open... easy.
-  - applys algo_trans (t_rcd l5 (A1|A2))...
-    + split_l; applys ASub_rcd. use_left_r... use_right_r...
-    + applys ASub_rcd. easy.
-Qed.
-
-Lemma nspli_isomorphic : forall A B1 B2,
-    new_spli A B1 B2 -> A ~~ B1&B2.
-Proof with eauto using ASub_refl.
-  introv Hs. induction Hs.
-  - split*.
-  - destruct IHHs.
-    split; applys algo_trans ((A1&A2)|B).
-    + match_or...
-    + match_and...
-    + match_and...
-    + match_or...
-  - destruct IHHs. split.
-    + applys algo_trans (A|B1&B2).
-      * match_or...
-      * swap_or_l... split_l.
-        use_right_r. swap_and_r...
-        use_right_r.
-        match_and_rev...
-        use_left_r. swap_and_r... use_left_r.
-        split_r...
-    + applys algo_trans (A|B1&B2).
-      * swap_or_r...
-        split_l. swap_and_l... split_l.
-        use_right_r. use_left_l...
-        use_right_l. use_right_r...
-        swap_and_l... split_l.
-        use_left_l. use_right_r...
-        use_left_r. match_and_rev...
-      * match_or...
-  - destruct IHHs. split; applys algo_trans (t_arrow A (B1&B2)).
-    + econstructor...
-    + match_and...
-    + split_r. eauto.
-      use_left_l...
-      use_right_l...
-    + econstructor...
-  - apply nsplu_isomorphic in H0.
-    destruct H0. split; applys algo_trans (t_arrow (A1|A2) B).
-    + econstructor...
-    + split_r; constructor~. use_left_r... use_right_r...
-    + convert2dsub. applys* DSub_FunDistI.
-    + constructor~.
-  - split; applys algo_trans (t_forall (A1&A2)).
-    + econstructor. intros. instantiate_cofinites. autorewrite with open. easy.
-    + split_r; econstructor; intros; autorewrite with open. use_left_l... use_right_l...
-    + convert2dsub. applys* DSub_CovDistIAll.
-    + econstructor. intros. instantiate_cofinites. autorewrite with open. easy.
-  - destruct IHHs. split; applys algo_trans (t_rcd l5 (A1&A2)).
-    + econstructor...
-    + match_and...
-    + split_r. eauto.
-      use_left_l...
-      use_right_l...
-    + econstructor...
-Qed.
-
-Lemma asub2nsub : forall A B,
-    algo_sub A B <-> new_sub A B.
-Proof with new_elia; try easy.
-  introv; split; intro H.
-  - induction H.
-    all: now eauto.
-  - indTypSize (size_typ A + size_typ B). inverts H.
-    1-3: eauto.
-    1,3-9: repeat match goal with
-                | H: new_sub _ _ |- _ => forwards~ : IH H; new_elia; clear H
-                  end.
-    + (* and *) applys~ algo_trans (B1&B2).
-      split_r...
-      forwards~ (?&?): nspli_isomorphic H0.
-    + (* andl *) applys~ algo_trans (A1&A2).
-      forwards~ (?&?): nspli_isomorphic H0.
-      use_left_l...
-    + (* andr *) applys~ algo_trans (A1&A2). forwards~ (?&?): nspli_isomorphic H0.
-      use_right_l...
-    + (* or *) applys~ algo_trans (A1|A2).
-      forwards~ (?&?): nsplu_isomorphic H0.
-      split_l...
-    + (* orl *) applys~ algo_trans (B1|B2). use_left_r...
-      forwards~ (?&?): nsplu_isomorphic H0.
-    + (* orr *) applys~ algo_trans (B1|B2). use_right_r...
-      forwards~ (?&?): nsplu_isomorphic H0.
-    + applys ASub_forall (L `union` [[A0]] `union` [[B0]]). intros X Fry.
-      instantiate_cofinites. applys~ IH; elia.
-Qed.
-
-(*********************** binding ********************************)
-
-Ltac close_typ_var X :=
-  repeat match goal with
-         | H: ?A = ?B -^ X |- _ =>
-           let H' := fresh "Heq" in
-           forwards~ H': close_typ_wrt_typ_open_typ_wrt_typ B;
-           rewrite <- H in H'; clear H
-         end.
-
-Ltac simpl_rename H :=
-  match type of H with
-  | context [ [?X ~~> _] (_ -^ ?X) ] =>
-    rewrite typsubst_typ_spec in H; rewrite close_typ_wrt_typ_open_typ_wrt_typ in H
-  | context [ [?X ~~> _] ?A ] =>
-    rewrite <- (open_typ_wrt_typ_close_typ_wrt_typ A X) in H;
-    rewrite typsubst_typ_spec in H; rewrite close_typ_wrt_typ_open_typ_wrt_typ in H
-  end.
-
-Ltac simpl_rename_goal :=
-  match goal with
-  | |- context [ [?X ~~> _] (_ -^ ?X) ] =>
-    rewrite typsubst_typ_spec; rewrite close_typ_wrt_typ_open_typ_wrt_typ
-  | |- context [ [?X ~~> _] ?A ] =>
-    rewrite <- (open_typ_wrt_typ_close_typ_wrt_typ A X);
-    rewrite typsubst_typ_spec; rewrite close_typ_wrt_typ_open_typ_wrt_typ
-  end.
-
-(* Aborted
-Lemma typsubst_typ_splu : forall A B C X U,
-    X `notin` [[A]] `union` [[B]] `union` [[C]] -> lc_typ U ->
-    new_splu ( A -^ X ) ( B -^ X ) ( C -^ X ) ->
-    new_splu ( A ^-^ U ) ( B ^-^ U ) ( C ^-^ U ).
-Proof with eauto with lngen.
-  introv Fry Lc Hs. inductions Hs; simpl.
-  - assert (Heq: (t_or B C) -^ X = t_or (B -^ X) (C -^ X)) by eauto.
-    rewrite <- Heq in x.
-    lets~ Heq2: open_typ_wrt_typ_inj x.
-    assert (Heq3: (t_or B C) ^-^ U = t_or (B ^-^ U) (C ^-^ U)) by eauto.
-    subst. rewrite Heq3. applys NSpU_or...
-  - close_typ_var X. subst.
-Abort. (* the following alternative definition is simpler *)
-*)
-Lemma typsubst_typ_splu : forall A B C X U,
-    new_splu A B C -> lc_typ U ->
-    new_splu ([X ~~> U] A) ([X ~~> U] B) ([X ~~> U] C).
-Proof with eauto with lngen.
-  introv spl lc. induction spl; simpl.
-  all: auto...
-  -
-    applys NSpU_forall (L `union` [[A]] `union` [[A1]] `union` [[A2]] `union` {{X}}).
-    intros Y Fry. instantiate_cofinites_with Y.
-    rewrite 3 typsubst_typ_open_typ_wrt_typ in H0...
-    rewrite (typsubst_typ_fresh_eq (t_tvar_f Y) U X) in H0...
-Qed.
-
-Lemma typsubst_typ_spli : forall A B C X U,
-    new_spli A B C -> lc_typ U ->
-    new_spli ([X ~~> U] A) ([X ~~> U] B) ([X ~~> U] C).
-Proof with eauto using typsubst_typ_splu with lngen.
-  introv spl lc. induction spl; simpl.
-  1-4, 7: auto...
-  - applys NSpI_arrowUnion...
-  - applys NSpI_forall (L `union` [[A]] `union` [[A1]] `union` [[A2]] `union` {{X}}).
-    intros Y Fry. instantiate_cofinites_with Y.
-    rewrite 3 typsubst_typ_open_typ_wrt_typ in H0...
-    rewrite (typsubst_typ_fresh_eq (t_tvar_f Y) U X) in H0...
-Qed.
-
-Lemma typsubst_typ_new_sub : forall A B C X,
-  new_sub A B -> lc_typ C ->
-  new_sub ([X ~~> C] A) ([X ~~> C] B).
-Proof with (simpl in *; eauto with lngen; eauto using typsubst_typ_lc_typ, typsubst_typ_spli, typsubst_typ_splu).
-  introv s lc.
-  indTypSize (size_typ A + size_typ B).
-  inverts s; simpl.
-  - applys NSub_refl...
-  - applys~ NSub_top...
-  - applys~ NSub_bot...
-  - applys~ NSub_arrow... all: applys IH; elia...
-  - applys~ NSub_forall (L `union` {{X}} `union` [[C]])...
-    intros Y HF. instantiate_cofinites_with Y.
-    rewrite 2 typsubst_typ_open_typ_wrt_typ_var...
-    applys IH; elia...
-  - applys~ NSub_rcd... applys IH; new_elia...
-  - applys~ NSub_and. applys typsubst_typ_spli H...
-    all: applys IH; new_elia...
-  - applys~ NSub_andl. applys typsubst_typ_spli H...
-    all: applys IH; new_elia...
-  - applys~ NSub_andr. applys typsubst_typ_spli H...
-    all: applys IH; new_elia...
-  - applys~ NSub_or. applys typsubst_typ_splu H...
-    all: applys IH; new_elia...
-  - applys~ NSub_orl. applys typsubst_typ_splu H...
-    all: applys IH; new_elia...
-  - applys~ NSub_orr. applys typsubst_typ_splu H...
-    all: applys IH; new_elia...
-Qed.
-
-(******** subtyping **********)
-
-
-Lemma typsubst_typ_algo_sub : forall A B C X,
-  algo_sub A B -> lc_typ C ->
-  algo_sub ([X ~~> C] A) ([X ~~> C] B).
-Proof.
-  intros.
-  apply asub2nsub. apply asub2nsub in H.
-  applys~ typsubst_typ_new_sub.
-Qed.
-
-Ltac solve_dsub := repeat match goal with
-                          | H: declarative_subtyping _ _ |- _ => apply dsub2asub in H
-                          | |- declarative_subtyping _ _ => apply dsub2asub
-                          end; try solve (solve_algo_sub).
-
-(*
-Lemma dsub_lc_1 : forall A B, declarative_subtyping A B -> lc_typ A.
-Proof.  introv H.  apply dsub2asub in H.  eauto.  Qed.
-
-Lemma dsub_lc_2 : forall A B, declarative_subtyping A B -> lc_typ B.
-Proof.  introv H.  apply dsub2asub in H. eauto.  Qed.
-
-#[export] Hint Immediate dsub_lc_1 dsub_lc_2 : core.
- *)
-
-Lemma sub_dec : forall A B,
-    lc_typ A -> lc_typ B -> declarative_subtyping A B \/ ~ (declarative_subtyping A B).
-Proof.
-  intros.
-  forwards~ [?|?]: decidability A B.
-  left. applys~ dsub2asub.
-  right. intro HF. apply dsub2asub in HF. eauto.
-Qed.
-
-Lemma nsub_splitu : forall A B B1 B2,
-    ~ declarative_subtyping B A -> splu B B1 B2 -> lc_typ A ->
-    ~ declarative_subtyping B1 A \/ ~ declarative_subtyping B2 A.
-Proof.
-  introv HN HS HL.
-  destruct (sub_dec B1 A); eauto.
-  destruct (sub_dec B2 A); eauto.
-  exfalso. applys HN.
-  apply dsub2asub in H, H0. applys~ dsub2asub.
-  split_l; eassumption.
-Qed.
-
-(******** appty **************)
 
 #[export]
 Hint Extern 0 =>
@@ -503,30 +22,30 @@ Ltac indTypFtySize s :=
 
 #[export] Hint Immediate orduFty_lc : core.
 
-Lemma nappty_lc_1 : forall A B, NApplyTy A B -> lc_typ A.
+Lemma napplyty_lc_1 : forall A B, NApplyTy A B -> lc_typ A.
 Proof.  introv H.  induction* H.  Qed.
 
-Lemma nappty_lc_2 : forall A B, NApplyTy A B -> lc_Fty B.
+Lemma napplyty_lc_2 : forall A B, NApplyTy A B -> lc_Fty B.
 Proof.  introv H.  induction* H.  Qed.
 
-#[export] Hint Immediate nappty_lc_1 nappty_lc_2 : core.
+#[export] Hint Immediate napplyty_lc_1 napplyty_lc_2 : core.
 
-Lemma appty_lc_1 : forall A B C, ApplyTy A B C -> lc_typ A.
+Lemma applyty_lc_1 : forall A B C, ApplyTy A B C -> lc_typ A.
 Proof.  introv H.  induction* H.  Qed.
 
-Lemma appty_lc_2 : forall A B C, ApplyTy A B C -> lc_Fty B.
+Lemma applyty_lc_2 : forall A B C, ApplyTy A B C -> lc_Fty B.
 Proof.  introv H.  induction* H. Qed.
 
-Lemma appty_lc_3 : forall A B C, ApplyTy A B C -> lc_typ C.
+Lemma applyty_lc_3 : forall A B C, ApplyTy A B C -> lc_typ C.
 Proof.  introv H.  induction~ H. inverts H. eauto with lngen. Qed.
 
-#[export] Hint Immediate appty_lc_1 appty_lc_2 appty_lc_3 : core.
+#[export] Hint Immediate applyty_lc_1 applyty_lc_2 applyty_lc_3 : core.
 
 (*
 Ltac solve_lc_by_regularity A :=
   match goal with
-  | H: ApplyTy _ _ _ |- _ => match type of H with context[ A ] => apply appty_lc in H end
-  | H: NApplyTy _ _ _ |- _ => match type of H with context[ A ] => apply nappty_lc in H end
+  | H: ApplyTy _ _ _ |- _ => match type of H with context[ A ] => apply applyty_lc in H end
+  | H: NApplyTy _ _ _ |- _ => match type of H with context[ A ] => apply napplyty_lc in H end
   end;
   destruct_conj.
 
@@ -534,7 +53,7 @@ Ltac solve_lc_by_regularity A :=
 #[export] Hint Extern 1 (lc_typ (?A -^ _) ) => progress solve_lc_by_regularity A : core.
  *)
 
-Lemma nappty_splitu_inv : forall A B B1 B2,
+Lemma napplyty_splitu_inv : forall A B B1 B2,
     NApplyTy A (fty_StackArg B) -> splu B B1 B2 ->
     NApplyTy A (fty_StackArg B1) \/ NApplyTy A (fty_StackArg B2).
 Proof.
@@ -542,7 +61,7 @@ Proof.
   inverts HN; solve_false; auto_unify; eauto.
 Qed.
 
-Lemma appty_contradication : forall A B C,
+Lemma applyty_contradication : forall A B C,
    ApplyTy A B C -> NApplyTy A B -> False.
 Proof with solve_false.
   introv HA HN.
@@ -551,7 +70,7 @@ Proof with solve_false.
   inverts HA;
     match goal with
     | H1: NApplyTy _ (fty_StackArg ?B), H2: splu ?B _ _  |- _ =>
-      forwards~ [?|?]: nappty_splitu_inv H1 H2
+      forwards~ [?|?]: napplyty_splitu_inv H1 H2
     | _ => inverts HN
     end.
 
@@ -565,10 +84,10 @@ Qed.
 
 #[export]  Hint Extern 1 => match goal with
                             | H1: ApplyTy ?T _ _, H2: NApplyTy ?T _  |- _ =>
-                              applys appty_contradication H1 H2
+                              applys applyty_contradication H1 H2
                             end : FalseHd.
 
-Lemma appty_unique : forall A B C1 C2,
+Lemma applyty_unique : forall A B C1 C2,
     ApplyTy A B C1 -> ApplyTy A B C2 -> C1 = C2.
 Proof.
   introv HA1 HA2. gen C1 C2.
@@ -582,10 +101,10 @@ Qed.
 
 Ltac auto_unify_2 :=
   auto_unify; (* unify split *)
-  (* unify appty *)
+  (* unify applyty *)
   repeat match goal with
          | [ H1: ApplyTy ?A ?B _ , H2: ApplyTy ?A ?B _ |- _ ] =>
-           (forwards : appty_unique H1 H2;
+           (forwards : applyty_unique H1 H2;
             subst; clear H2)
              end.
 
@@ -597,35 +116,33 @@ Proof.
   forwards* [?|(?&?&?)]: ordu_or_split A.
 Qed.
 
-Lemma appty_total : forall A F,
-    lc_typ A -> lc_Fty F -> exists C, ApplyTy A F C \/ NApplyTy A F.
-Proof.
+Lemma applyty_total : forall A F,
+    lc_typ A -> lc_Fty F -> (exists C, ApplyTy A F C) \/ NApplyTy A F.
+Proof with (elia; destruct_conj).
   introv.
   indTypFtySize (size_typ A + size_Fty F).
   lets~ [?|(?&?&?&?&?)]: (ordu_or_split_Fty F).
   - destruct* H.
     (* and / or *)
-    all: try forwards~ (?&[?|?]): IH F A1; elia.
-    all: try forwards~ (?&[?|?]): IH F A2; elia.
+    all: try forwards~ [?|?]: IH F A1...
+    all: try forwards~ [?|?]: IH F A2...
     all: eauto.
 
     (* arrow / forall *)
     all: destruct H0.
-    2,3: solve [exists; right*].
+    2,3: now right*.
 
     + destruct* (sub_dec A0 A).
     + eauto.
 
   - subst.
-    forwards~ (?&[?|?]): IH (fty_StackArg x0) A; elia.
-    forwards~ (?&[?|?]): IH (fty_StackArg x1) A; elia.
+    forwards~ [?|?]: IH (fty_StackArg x0) A...
+    forwards~ [?|?]: IH (fty_StackArg x1) A...
     all: eauto.
-
-  Unshelve. all: apply t_top.
 Qed.
 
 
-Lemma appty_splitu_arg_inv : forall A B B1 B2 C,
+Lemma applyty_splitu_arg_inv : forall A B B1 B2 C,
     ApplyTy A (fty_StackArg B) C -> splu B B1 B2 ->
     exists C1 C2, C = (t_or C1 C2) /\
     ApplyTy A (fty_StackArg B1) C1 /\ ApplyTy A (fty_StackArg B2) C2.
@@ -635,7 +152,7 @@ Proof.
 Qed.
 
 
-Lemma appty_splitu_fun_aux : forall A A1 A2 F,
+Lemma applyty_splitu_fun_aux : forall A A1 A2 F,
     (forall C1 C2, ApplyTy A1 F C1 -> ApplyTy A2 F C2 -> splu A A1 A2 ->
      exists C', ApplyTy A F C') /\
     (NApplyTy A1 F \/ NApplyTy A2 F -> splu A A1 A2 -> NApplyTy A F).
@@ -664,7 +181,7 @@ Proof with elia; solve_false; try eassumption.
     + (* forall *) inverts HA1... inverts HA2... exists*.
     + (* rcd *) inverts HA1...
   - subst.
-    forwards: appty_splitu_arg_inv HA1 H0. forwards: appty_splitu_arg_inv HA2 H0.
+    forwards: applyty_splitu_arg_inv HA1 H0. forwards: applyty_splitu_arg_inv HA2 H0.
     destruct_conj. subst.
     forwards (?&?): proj1 (IH (fty_StackArg x0) A) H4 H2...
     forwards (?&?): proj1 (IH (fty_StackArg x1) A) H5 H3...
@@ -677,143 +194,44 @@ Proof with elia; solve_false; try eassumption.
       * (* and *) inverts HA... forwards~ : proj2 (IH F A0) H1...
       * (* and *) inverts HA... forwards~ : proj2 (IH F B) H1...
       * (* forall *) inverts HA... constructor~.
-    + (* split *) forwards* [?|?]: nappty_splitu_inv HA.
+    + (* split *) forwards* [?|?]: napplyty_splitu_inv HA.
       * forwards~ : proj2 (IH (fty_StackArg x0) A) HS... eauto.
       * forwards~ : proj2 (IH (fty_StackArg x1) A) HS... eauto.
     + (* ord *) inverts~ HS...
       * (* and *) inverts HA... forwards~ : proj2 (IH F A0) H1...
       * (* and *) inverts HA... forwards~ : proj2 (IH F B) H1...
       * (* forall *) inverts HA... constructor~.
-    + (* split *) forwards* [?|?]: nappty_splitu_inv HA.
+    + (* split *) forwards* [?|?]: napplyty_splitu_inv HA.
       * forwards~ : proj2 (IH (fty_StackArg x0) A) HS... eauto.
       * forwards~ : proj2 (IH (fty_StackArg x1) A) HS... eauto.
 
    Unshelve. all: apply t_top.
 Qed.
 
-Lemma appty_splitu_fun : forall A A1 A2 F C1 C2,
-    ApplyTy A1 F C1 -> ApplyTy A2 F C2 -> splu A A1 A2 ->
-    exists C', ApplyTy A F C' /\ declarative_subtyping C' (t_or C1 C2).
-Proof.
-  intros.
-  forwards* (?&?): appty_splitu_fun_aux.
-Abort.
-
-Lemma nappty_splitu_fun : forall A A1 A2 F,
+Lemma napplyty_splitu_fun : forall A A1 A2 F,
     NApplyTy A1 F \/ NApplyTy A2 F -> splu A A1 A2 -> NApplyTy A F.
 Proof.
   intros.
-  forwards* (?&?): appty_splitu_fun_aux.
+  forwards* (?&?): applyty_splitu_fun_aux.
 Qed.
-(*
-Lemma nappty_split_inv : forall A A1 A2 F,
-    NApplyTy A F -> spli A A1 A2 -> NApplyTy A1 F /\ NApplyTy A2 F.
-Proof with elia; try eassumption; eauto.
-  introv HN HS.
-  indTypFtySize (size_typ A + size_Fty F).
-  inverts HN; solve_false.
-  - (* rcd *) inverts HS; eauto.
-  - (* forall *) inverts HS. split; constructor~.
-  - (* arrow sub *) inverts~ HS.
-    assert (~ declarative_subtyping B A3). {
-      intros HF. apply H2. solve_dsub.
-    }
-    assert (~ declarative_subtyping B A4). {
-      intros HF. apply H2. solve_dsub.
-    }
-    eauto.
-  - (* arrow *) inverts~ HS.
-  - (* or *) forwards [ [?|?] | [?|?] ]: double_split HS. eauto.
-    all: destruct_conj.
-    all: try match goal with
-             | H1: NApplyTy ?A _, H2: spli ?A _ _ |- _ => forwards (?&?): IH H1 H2; elia
-             end.
-    all: split*.
-    all: applys nappty_splitu_fun; try eassumption; eauto.
-  - (* or *) forwards [ [?|?] | [?|?] ]: double_split HS. eauto.
-    all: destruct_conj.
-    all: try match goal with
-             | H1: NApplyTy ?A _, H2: spli ?A _ _ |- _ => forwards (?&?): IH H1 H2; elia
-             end.
-    all: split*.
-    all: applys nappty_splitu_fun...
-  - (* union argL *)
-    split.
-    all: applys NApplyTyUnionArgL...
-    all: applys IH HS...
-  - (* union argR *)
-    split.
-    all: applys NApplyTyUnionArgR...
-    all: applys IH HS...
-  - auto_unify...
 
-    Unshelve. all: apply t_top.
-Abort.
-*)
-(* this definition cannot work
-Lemma appty_split_inv : forall A A1 A2 F C,
-    ApplyTy A F C -> spli A A1 A2 -> UnionOrdinaryFty F ->
-    exists C1 C2,
-    (ApplyTy A1 F C1 /\ C <: C1) \/ ApplyTy A2 F C2.
- *)
-
-Lemma appty_split_inv : forall A A1 A2 F C,
-    ApplyTy A F C -> spli A A1 A2 -> UnionOrdinaryFty F ->
-    (exists C1 C2, ApplyTy A1 F C1 /\ ApplyTy A2 F C2 /\ (t_and C1 C2) <: C) \/
-    ApplyTy A1 F C \/ ApplyTy A2 F C.
-(*    (ApplyTy A1 F C /\ NApplyTy A2 F \/ ApplyTy A2 F C /\ NApplyTy A2 F ). *)
-Proof with elia; try eassumption; eauto.
-  introv HA HS HU.
-  indTypFtySize (size_typ A).
-  inverts HA; solve_false; auto_unify...
-  - (* forall *) inverts HS; eauto.  Abort. (*
-  - (* arrow sub *) inverts~ HS.
-    + left*.
-    + inverts keep H0.
-      solve_dsub. forwards [?|?]: algo_sub_orlr_inv H1...
-      * left. exists. applys~ ApplyTyFun. solve_dsub...
-      * right. exists. applys~ ApplyTyFun. solve_dsub...
-  - (* or *) forwards [ [?|?] | [?|?] ]: double_split HS. eauto.
-    all: destruct_conj.
-    all: repeat match goal with
-             | H1: ApplyTy ?A _ _, H2: spli ?A _ _ |- _ =>
-               forwards [(?&?)|(?&?)]: IH H2 H1; elia; clear H2
-             | H1: ApplyTy ?A1 _ _, H2: ApplyTy ?A2 _ _, H3: splu _ ?A1 ?A2 |- _ =>
-               forwards* (?&?): appty_splitu_fun H1 H2 H3; elia; clear H3
-                end.
-    all: eauto.
-Qed. *)
-(*
-The above lemma does not hold without ordu condition
-
-Let B1 B2 be two ordu types
-
-apply (A1, B1) => apply (A1&A2, B1)
-apply (A2, B2) => apply (A1&A2, B2)
-
-together we have apply (A1&A2, B1 | B2)
-
-But neither apply (A1, B1|B2) or apply (A2, B1|B2) holds
- *)
-
-
-Lemma nappty_rename : forall A B C,
+Lemma napplyty_rename : forall A B C,
     NApplyTy A (fty_StackTyArg B) -> lc_typ C -> NApplyTy A (fty_StackTyArg C).
 Proof.
   introv H Lc. inductions H; eauto.
 Qed.
 
-Lemma appty_rename : forall A B X C,
+Lemma applyty_rename : forall A B X C,
     ApplyTy A (fty_StackTyArg (t_tvar_f X)) B -> lc_typ C -> X `notin` [[A]] ->
     ApplyTy A (fty_StackTyArg C) ( [X ~~> C] B).
 Proof.
   introv H Lc Fry. inductions H; simpl; simpl in Fry; eauto.
   all: try solve [ simpl_rename_goal; simpl in Fry; solve_notin ].
-  - forwards~: nappty_rename C H1.
-  - forwards~: nappty_rename C H0.
+  - forwards~: napplyty_rename C H1.
+  - forwards~: napplyty_rename C H0.
 Qed.
 
-Lemma appty_soundness_1 : forall A B C,
+Lemma applyty_soundness_1 : forall A B C,
     ApplyTy A (fty_StackArg B) C -> A <: (t_arrow B C).
 Proof with try eassumption; try applys ASub_refl; try match goal with |- lc_typ _ => eauto with lngen end.
   introv H. inductions H.
@@ -839,7 +257,7 @@ Proof with try eassumption; try applys ASub_refl; try match goal with |- lc_typ 
   - convert2asub. split_r; eauto.
 Qed.
 
-Lemma appty_soundness_2 : forall A B C,
+Lemma applyty_soundness_2 : forall A B C,
     ApplyTy A (fty_StackTyArg B) C ->
     exists C',  C = C'^-^B /\
                 forall X, X `notin` [[C]] -> ApplyTy A (fty_StackTyArg (t_tvar_f X)) (C'-^X) /\ A <: (t_forall C').
@@ -863,10 +281,10 @@ Proof with simpl in *; try eassumption; try applys ASub_refl; try match goal wit
       * convert2asub.
         split_l. use_left_r...  use_right_r...
   - exists. split... intros X Fry. forwards~ : H2 X...
-    split. eapply nappty_rename in H1. eauto. eauto.
+    split. eapply napplyty_rename in H1. eauto. eauto.
     convert2asub. use_left_l...
   - exists. split... intros X Fry. forwards~ : H2 X...
-    split. eapply nappty_rename in H0. eauto. eauto.
+    split. eapply napplyty_rename in H0. eauto. eauto.
     convert2asub. swap_and_l... use_left_l...
   - exists (x0 & x). split...
     + assert (Heq: forall B C X, (t_and B C) ^-^ X = t_and (B ^-^ X) (C ^-^ X)) by eauto.
@@ -879,7 +297,7 @@ Proof with simpl in *; try eassumption; try applys ASub_refl; try match goal wit
   Unshelve. all: apply empty.
 Qed.
 
-Lemma appty_completeness_1 : forall A B D,
+Lemma applyty_completeness_1 : forall A B D,
     A <: (t_arrow B D) -> ordu B ->
          exists C, ApplyTy A (fty_StackArg B) C /\ (t_arrow B C) <: (t_arrow B D).
 Proof with try eassumption; elia; solve_false; destruct_conj.
@@ -890,12 +308,12 @@ Proof with try eassumption; elia; solve_false; destruct_conj.
   - destruct H...
     + forwards~ [Ha|Ha]: algo_sub_andlr_inv HS;
         forwards: IH Ha...
-      * forwards~ (?&[?|?]): appty_total A2 (fty_StackArg B).
+      * forwards~ [?|?]: applyty_total A2 (fty_StackArg B)...
         inv_arrow.
         exists (t_and x x0). split~. applys~ DSub_CovArr. applys~ DSub_InterLL.
         eauto with lngen. solve_dsub...
         exists* x.
-      * forwards~ (?&[?|?]): appty_total A1 (fty_StackArg B).
+      * forwards~ [?|?]: applyty_total A1 (fty_StackArg B)...
         inv_arrow.
         exists (t_and x0 x). split~. applys~ DSub_CovArr. applys~ DSub_InterLR.
         eauto with lngen. solve_dsub...
@@ -914,21 +332,7 @@ Proof with try eassumption; elia; solve_false; destruct_conj.
      convert2asub. eauto.
 Qed.
 
-(* hard to define with current definition *)
-(*)
-Lemma appty_completeness_2 : forall A B,
-    A <: (t_forall B) ->
-         exists C, ApplyTy A (fty_StackTyArg B) C /\ C[B~>X]?? <: (t_forall B).
-*)
-
-(* no determinism if defined in this way
-
-  ------------------------------------ :: ApplyFunTy
-  apply(forall X . A, [B]) => A
- *)
-
-
-Lemma appty_completeness_2 : forall A B,
+Lemma applyty_completeness_2 : forall A B,
     A <: (t_forall B) ->
          exists C L, forall X, X `notin` L ->
              ApplyTy A (fty_StackTyArg (t_tvar_f X)) (C-^X) /\ (t_forall C) <: (t_forall B).
@@ -940,9 +344,9 @@ Proof with try eassumption; elia; solve_false; destruct_conj.
     + forwards~ [Ha|Ha]: algo_sub_andlr_inv HS;
         forwards: IH Ha...
       * pick fresh X for ([[A1]] `union` [[A2]] `union` x0 `union` [[x]]). forwards~ : H0 X.
-        forwards~ (?&[?|?]): appty_total A2 (fty_StackTyArg (t_tvar_f X)); destruct_conj.
+        forwards~ [?|?]: applyty_total A2 (fty_StackTyArg (t_tvar_f X))...
         ** exists. intros Y Fry.
-           forwards~ HR1: appty_rename (t_tvar_f Y) H1. forwards~ HR2: appty_rename (t_tvar_f Y) H2.
+           forwards~ HR1: applyty_rename (t_tvar_f Y) H1. forwards~ HR2: applyty_rename (t_tvar_f Y) H2.
            simpl_rename HR1. simpl_rename HR2.
            assert (Heq: forall Y, (t_and x (close_typ_wrt_typ X x1)) -^ Y = t_and (x -^ Y) (close_typ_wrt_typ X x1 -^ Y)) by eauto. rewrite Heq.
            split~. applys DSub_CovAll. intros X0 Fry2.
@@ -951,13 +355,13 @@ Proof with try eassumption; elia; solve_false; destruct_conj.
            solve_dsub...
            autorewrite with lngen. all: solve_notin.
         ** exists. intros Y Fry.
-           forwards~ HR1: appty_rename (t_tvar_f Y) H1. simpl_rename HR1.
-           forwards~ HR2: nappty_rename (t_tvar_f Y) H2.
+           forwards~ HR1: applyty_rename (t_tvar_f Y) H1. simpl_rename HR1.
+           forwards~ HR2: napplyty_rename (t_tvar_f Y) H2.
            split. applys~ ApplyTyInterL HR1. auto. eauto with lngen.
       * pick fresh X for ([[A1]] `union` [[A2]] `union` x0 `union` [[x]]). forwards~ : H0 X.
-        forwards~ (?&[?|?]): appty_total A1 (fty_StackTyArg (t_tvar_f X)); destruct_conj.
+        forwards~ [?|?]: applyty_total A1 (fty_StackTyArg (t_tvar_f X))...
         ** exists. intros Y Fry.
-           forwards~ HR1: appty_rename (t_tvar_f Y) H1. forwards~ HR2: appty_rename (t_tvar_f Y) H2.
+           forwards~ HR1: applyty_rename (t_tvar_f Y) H1. forwards~ HR2: applyty_rename (t_tvar_f Y) H2.
            simpl_rename HR1. simpl_rename HR2.
            assert (Heq: forall Y, (t_and (close_typ_wrt_typ X x1) x) -^ Y = t_and (close_typ_wrt_typ X x1 -^ Y) (x -^ Y)) by eauto. rewrite Heq.
            split~. applys DSub_CovAll. intros X0 Fry2.
@@ -967,8 +371,8 @@ Proof with try eassumption; elia; solve_false; destruct_conj.
            autorewrite with lngen.
            all : solve_notin.
         ** exists. intros Y Fry.
-           forwards~ HR1: appty_rename (t_tvar_f Y) H1. simpl_rename HR1.
-           forwards~ HR2: nappty_rename (t_tvar_f Y) H2.
+           forwards~ HR1: applyty_rename (t_tvar_f Y) H1. simpl_rename HR1.
+           forwards~ HR2: napplyty_rename (t_tvar_f Y) H2.
            split. applys~ ApplyTyInterR HR1. auto. eauto with lngen.
 
     + apply dsub2asub in HS.
@@ -1000,28 +404,28 @@ Proof with try eassumption; elia; solve_false; destruct_conj.
 Qed.
 
 
-Lemma monotonicity_appty_1 : forall A A' F C,
+Lemma monotonicity_applyty_1 : forall A A' F C,
     ApplyTy A F C -> A' <: A -> exists C', C' <: C /\ ApplyTy A' F C'.
 Proof with try eassumption; elia; solve_false; destruct_conj.
   introv HA HS.
   indTypFtySize (size_typ A' + size_typ A + size_Fty F).
   lets~ [HF|(?&?&?&?&?)]: (ordu_or_split_Fty F). eauto.
-  2: { subst. forwards : appty_splitu_arg_inv HA H0. destruct_conj.
+  2: { subst. forwards : applyty_splitu_arg_inv HA H0. destruct_conj.
        subst. forwards (?&?&?): IH H1... forwards (?&?&?): IH H2...
        exists. split. 2: applys~ ApplyTyUnionArg H0...
        applys~ DSub_UnionL. }
   inverts HF.
-  - forwards: appty_soundness_1 HA.
+  - forwards: applyty_soundness_1 HA.
     forwards HSN: DSub_Trans HS...
-    forwards~ : appty_completeness_1 HSN. destruct_conj.
+    forwards~ : applyty_completeness_1 HSN. destruct_conj.
     inv_arrow. convert2dsub. exists* x.
-  - forwards: appty_soundness_2 HA...
+  - forwards: applyty_soundness_2 HA...
     pick_fresh Y. forwards~ : H1 Y...
     forwards HSN: DSub_Trans HS...
-    forwards~ : appty_completeness_2 HSN...
+    forwards~ : applyty_completeness_2 HSN...
     pick fresh X.
     forwards~ : H4 X. destruct_conj.
-    eapply appty_rename in H5. exists. split...
+    eapply applyty_rename in H5. exists. split...
     simpl_rename_goal. subst~.
     convert2asub.
     forwards : algo_sub_forall_inv X H6.
@@ -1032,16 +436,16 @@ Proof with try eassumption; elia; solve_false; destruct_conj.
     all: eauto.
 Qed.
 
-Lemma monotonicity_appty_2_1 : forall A B B' C,
+Lemma monotonicity_applyty_2_1 : forall A B B' C,
     ApplyTy A (fty_StackArg B) C -> declarative_subtyping B' B ->
     exists C', declarative_subtyping C' C /\ ApplyTy A (fty_StackArg B') C'.
 Proof with try eassumption; elia; solve_false; destruct_conj.
   introv HA HS.
   indTypFtySize (size_typ A + size_typ B' + size_typ B).
   lets~ [HF|(?&?&?)]: (ordu_or_split B').
-  - forwards: appty_soundness_1 HA.
+  - forwards: applyty_soundness_1 HA.
     forwards HSN: DSub_Trans H... applys DSub_FunCon HS. eauto.
-    forwards~ : appty_completeness_1 HSN. destruct_conj.
+    forwards~ : applyty_completeness_1 HSN. destruct_conj.
     inv_arrow. convert2dsub. exists* x.
   - assert (S1: x <: B). {
       applys~ DSub_Trans HS.
@@ -1055,60 +459,3 @@ Proof with try eassumption; elia; solve_false; destruct_conj.
     forwards: IH S2...
     exists (x1|x2). split~. applys~ ApplyTyUnionArg H.
 Qed.
-
-Lemma monotonicity_subtyping : forall A B C D X,
-  algo_sub A B -> algo_sub C D ->
-  algo_sub ([X ~~> C] A) ([X ~~> D] B).
-Proof with (simpl in *; eauto with lngen; eauto using typsubst_typ_lc_typ, typsubst_typ_spli, typsubst_typ_splu).
-  introv HS1 HS2.
-  applys algo_trans [X ~~> C] (B).
-  { applys* typsubst_typ_algo_sub. }
-  assert (Lc: lc_typ B) by eauto.
-  clear HS1.
-  convert2dsub.
-  induction Lc; simpl; auto.
-  - case_if; auto.
-  - applys DSub_Trans (t_arrow [X ~~> C] (A0) [X ~~> D] (B)).
-    + applys~ DSub_CovArr.
-    + applys~ DSub_FunCon.
-      (* incorrect lemma: breaks in function case *)
-Abort.
-(*   IHLc1 : [X ~~> C] (A0) <: [X ~~> D] (A0)
-  IHLc2 : [X ~~> C] (B) <: [X ~~> D] (B)
-  ============================
-  [X ~~> D] (A0) <: [X ~~> C] (A0)
- *)
-
-Lemma monotonicity_appty_2_2 : forall A B B' C,
-    ApplyTy A (fty_StackTyArg B) C -> declarative_subtyping B' B ->
-    exists C', declarative_subtyping C' C /\ ApplyTy A (fty_StackTyArg B') C'.
-Proof with try eassumption; elia; solve_false; destruct_conj.
-  introv HA HS.
-  forwards: appty_soundness_2 HA. destruct_conj.
-  subst.
-  pick fresh X. forwards~ (?&HS2): H0 X.
-  { forwards Hless: typefv_typ_open_typ_wrt_typ_upper x B.
-    rewrite Hless. solve_notin. }
-  forwards (y&?&?): appty_completeness_2 HS2.
-  exists (y ^-^ B').
-  pick fresh Y. forwards~ (Happ&?): H1 Y.
-  forwards~ HG: appty_rename B' Happ.
-  simpl_rename HG. split~.
-  { convert2asub. forwards: algo_sub_forall_inv Y H2.
-    Abort. (*
-    forwards: monotonicity_subtyping Y H3 HS.
-    repeat simpl_rename H4. all: auto. }
-  solve_notin.
-Qed. *)
-
-(*
-C <: B
-
-apply ( forall X . X -> A  , [ B ] ) => B -> A
-
-apply ( forall X . X -> A  , [ C ] ) => C -> A
-
-=======================================================
-
-XXX   C -> A <: B -> A   XXX
-*)
